Added bounded version of top-level constraint checker.

checker/coq/model.v
@@ -8,6 +8,10 @@ Require Import bounds.
 Require Import sol.
 Require Import arith.
 
+Require Import linear_dset.
+Require Import element_dset.
+Require Import cumul_dset.
+
 (* Closed set of constraints. *)
 Inductive cst :=
   | Lin : LinearCon.(T) -> cst
@@ -27,10 +31,25 @@ Definition eval_cst c theta := match c with
   | Arith x => ArithConstraint.(eval) x theta
   end.
 
+Definition eval_cst_bnd b c theta :=
+  match c with
+  | Lin x => eval LinearDSet (b, x) theta                                            
+  | Elem x => eval ElemDbnd (b, x) theta                                            
+  | Cumul x => eval CumulDomBnd (b, x) theta                                            
+  | Clause x => eval (DomboundedConstraint ClauseCon) (b, x) theta
+  | Arith x => eval ArithDbnd (b, x) theta
+  end.
+
 Fixpoint eval_csts (cs : csts) theta := 
   match cs with
   | nil => True
   | cons c cs' => (eval_cst (snd c) theta) /\ (eval_csts cs' theta)
+  end.
+
+Definition eval_csts_bnd b cs theta :=
+  match cs with
+  | nil => True
+  | cons c cs' => (eval_cst_bnd b (snd c) theta) /\ (eval_csts cs' theta)
   end.
 
 Definition model := ((list model_bound) * csts)%type.
@@ -61,6 +80,16 @@ Definition check_cst (c : cst) (cl : clause) :=
   | Arith x => check ArithConstraint ArithCheck x cl
   end.
 
+Definition check_cst_bnd b (c : cst) (cl : clause) :=
+  match c with
+  | Lin x => check LinearDSet LinearDBCheck (b, x) cl
+  | Elem x => check ElemDbnd ElemDomCheck (b, x) cl
+  | Cumul x => check CumulDomBnd CumulTTDCheck (b, x) cl
+  | Arith x => check ArithDbnd ArithDomCheck (b, x) cl
+  (* GKG: FIXME *)
+  | Clause x => check ClauseCon CheckClause x cl
+  end.
+
 Theorem check_cst_valid : forall (c : cst) (cl : clause),
   check_cst c cl = true ->
     forall theta, eval_cst c theta -> eval_clause cl theta.
@@ -72,4 +101,17 @@ Proof.
      apply (check_valid ClauseCon CheckClause t cl) in H |
      apply (check_valid ArithConstraint ArithCheck t cl) in H ];
   unfold implies in H; try apply H; try apply H0.
+Qed.
+
+Theorem check_cst_bnd_valid : forall (b : domset) (c : cst) (cl : clause),
+  check_cst_bnd b c cl = true ->
+    forall theta, eval_domset b theta -> eval_cst c theta -> eval_clause cl theta.
+Proof.
+  unfold eval_cst, check_cst_bnd; destruct c; intros;
+  [apply (check_valid LinearDSet LinearDBCheck (b, t) cl) |
+   apply (check_valid ElemDbnd ElemDomCheck (b, t) cl) |
+   apply (check_valid CumulDomBnd CumulTTDCheck (b, t) cl) |
+   apply (check_valid ClauseCon CheckClause t cl) |
+   apply (check_valid ArithDbnd ArithDomCheck (b, t) cl) ];
+  try assumption; try (apply eval_dombounded_if; assumption).
 Qed.
